@prefix : <http://vocab.ub.uni-leipzig.de/diggr/> .
@prefix diggr: <http://vocab.ub.uni-leipzig.de/diggr/> .
@prefix rdf: <http://www.w3.org/1999/02/22-rdf-syntax-ns#> .
@prefix rdfs: <http://www.w3.org/2000/01/rdf-schema#>.
@prefix owl: <http://www.w3.org/2002/07/owl#>.
@prefix VideoGameOntology: <http://purl.org/net/VideoGameOntology#> .
@prefix xsd: <http://www.w3.org/2001/XMLSchema#> .
@prefix terms: <http://purl.org/dc/terms/> .
@prefix vann: <http://purl.org/vocab/vann/> .
@prefix doap: <http://usefulinc.com/ns/doap#> .
@prefix gndo: <http://d-nb.info/standards/elementset/gnd#> .
@prefix frbroo: <http://iflastandards.info/ns/fr/frbr/frbroo/> .
@prefix crm: <http://www.cidoc-crm.org/cidoc-crm/> .
@prefix dbo: <http://dbpedia.org/ontology/> .
@prefix rcgs: <http://www.rcgs.jp/terms/> .
@prefix dct:   <http://purl.org/dc/terms/> .
@base <http://vocab.ub.uni-leipzig.de/diggr/> .

<http://vocab.ub.uni-leipzig.de/diggr/> a <http://purl.org/vocommons/voaf#Vocabulary>, owl:Ontology ;
    rdfs:label "diggr Video Game Vocabulary"@en ;
     dbo:subtitle "A Vocabulary for Interlinking Video Game Databases"@en ;
     vann:preferredNamespacePrefix "diggr" ;
     vann:preferredNamespaceUri "http://vocab.ub.uni-leipzig.de/diggr/" ;
     owl:versionInfo "1.1" ;
	 dct:creator "Tracy Hoffmann" ;
     terms:modified "2019-02-15"^^xsd:date ;
     terms:created "2017-04-04"^^xsd:date ;
     terms:license "CC0 1.0 Universal";
     doap:homepage <http://diggr.link> .

######################## Classes #####################################

diggr:DiggrEntity rdf:type owl:Class ;
	rdfs:subClassOf owl:Thing , crm:E1_CRM_Entity ;
	rdfs:comment "Comprises all game related things."@en ;                    
    rdfs:label "Diggr Game Entity"@en .

## Main Game Classes

diggr:Game a owl:Class;
	rdfs:subClassOf diggr:DiggrEntity, frbroo:F1_Work, rcgs:Work;
	owl:equivalentClass VideoGameOntology:Game ;
	rdfs:comment """The Game entity type is an abstract entity that describes features that are shared among different editions of a game.
		The characteristics that are typically recognized by users when they say “we played the same game” even if they played it on different platforms (e.g. PlayStations 3 and Xbox 360).
		Features attributed to the Game entity type also support distinguishing between games by genre, mood, theme, setting, plot, etc."""@en ;
	rdfs:label "Videospiel"@de , "Video Game"@en .

diggr:Platform_Realization a owl:Class;
	rdfs:subClassOf diggr:DiggrEntity, frbroo:F22_Self-Contained_Expression, rcgs:Variation;
	rdfs:comment """The Platform Realization class denotes a particular instantiation of a video game from a technical perspective.
		It differs in the development for a particular hardware platform (e.g. PlayStation 3 or Xbox 360).
		The Platform Realization bundles together such features as special additional hardware or system requirements.
		A Platform Realization differs to others on the basis of a certain platform and thus by major differences in the program code. A port creates a new platform edition entity."""@en ; 
	rdfs:label "Plattform Realisation"@de , "Platform Realization"@en . 

diggr:Generic_Edition a owl:Class;
	rdfs:subClassOf diggr:DiggrEntity, frbroo:F24_Publication_Expression, rcgs:Variation ;
	rdfs:comment """The Generic Edition is the creative or economic vision of game which will be realized in Platform Realizations.
		The Edition denotes a particular instantiation of a video game from a publisher or distributional perspective.
		"""@en ;
	rdfs:label "Ausgabe (generisch)"@de , "Edition (generic)"@en . 

diggr:Special_Edition a owl:Class;
	rdfs:subClassOf diggr:Generic_Edition ;
	rdfs:comment """A Special Edition may be a particular release of a game that is in some way different than another release of the same game on the same platform.
		This may be because it has fully integrated content that was previously available only as separate expansion material or additional content/features not available in the regular edition of the game. 
		This can also be done in physical form e.g. with merchandise."""@en ;
	rdfs:label "Ausgabe (speziell)"@de , "Edition (special)"@en . 

diggr:LocalRelease a owl:Class;
	rdfs:subClassOf diggr:DiggrEntity, frbroo:F3_Manifestation_Product_Type, rcgs:Package ;
	rdfs:comment """A Local Release incorporates a specific Edition and a specific Platform Realization.
		It is made available and accessible in a particular region and in a particular language.
		Local releases can differ in language, graphics localization, customization options for difficulty levels and characters."""@en ;
	rdfs:label "Lokale Veröffentlichung"@de , "Local Release"@en . 

## Additional Classes

diggr:Platform a owl:Class;
	rdfs:subClassOf diggr:DiggrEntity, rcgs:Platform ;
	rdfs:comment "Hardware or Software platform for which a Video Game is developed or released e.g. PlayStation 2 or XBox One."@en ; 
	rdfs:label "Plattform"@de , "Platform"@en .  

diggr:ProductionEvent a owl:Class;
	rdfs:subClassOf crm:E5_Event ;
#	rdfs:subClassOf
#              [ a       owl:Restriction ;
#                owl:allValuesFrom diggr:RoleRelation ;
#                owl:onProperty diggr:hasContributor
#              ] ;
	rdfs:comment "The act of creating a video game."@en ;   
	rdfs:label "Produktionsevent"@de , "Production event"@en .

diggr:Role a owl:Class;
	rdfs:comment "A role within a game production process, e.g. writer, developer, voice actor, etc."@en ;
	rdfs:label "Rolle"@de , "Role"@en . 

diggr:Company a owl:Class ;
	rdfs:subClassOf crm:E39_Actor ;
    rdfs:comment "A company which is involved in the video game industry."@en ;
	rdfs:label "Firma"@de , "Company"@en . 

## Helper Classes

diggr:RoleRelation a owl:Class ;
    rdfs:comment "An role relation connects actors (persons or companies) and their roles inside the video game production."@en ;
	rdfs:label "Rolenrelation"@de , "Role relation"@en .
#    rdfs:subClassOf
#              [ a       owl:Restriction ;
#                owl:allValuesFrom diggr:Role ;
#                owl:onProperty diggr:roleValue
#              ] ;
#    rdfs:subClassOf
#              [ a       owl:Restriction ;
#                owl:allValuesFrom crm:E39_Actor ;
#                owl:onProperty diggr:roleActor
#              ] .

diggr:LocationStatement a owl:Class ;
    rdfs:comment "A location statement connects places or geographic entities with time or time span."@en ;
	rdfs:label "Ortsangabe"@de , "Location statement"@en .

######################## Properties #####################################

diggr:hasContributor a owl:ObjectProperty ;
   rdfs:domain diggr:ProductionEvent ;
   rdfs:range diggr:RoleRelation ;
   rdfs:comment "A game production event has one or more contributors, e.g. writers, developers, voice actors, etc. which are defined by a role relation."@en ;
   rdfs:label "has contributor"@en .

diggr:roleActor a owl:ObjectProperty ;
   rdfs:domain diggr:RoleRelation ;
   rdfs:range crm:E39_Actor ;
   rdfs:comment "An actor has one or more roles within a game production process, e.g. writers, developers, voice actors, etc. and can also be a company."@en ;
   rdfs:label "role actor"@en .

diggr:roleValue a owl:ObjectProperty ;
   rdfs:domain diggr:RoleRelation ;
   rdfs:range diggr:Role ;
   rdfs:comment "A game production role, e.g. writer, developer, voice actors, etc."@en ;
   rdfs:label "role value"@en .

diggr:worksFor a owl:ObjectProperty ;
   rdfs:domain diggr:RoleRelation ;
   rdfs:range crm:E39_Actor ;
   rdfs:comment "The relation between a specific role, actor and a corporation at the point in time of the production process."@en ;
   rdfs:label "works for/cooperate with"@en .

diggr:createdBy a owl:ObjectProperty ;
	rdfs:range diggr:ProductionEvent ;
	rdfs:comment "A platform realization is created during an production event."@en ;
	rdfs:label "is created by"@en .

diggr:isDeveloperOf a owl:ObjectProperty ;
	rdfs:domain diggr:Company ;
	rdfs:range diggr:Platform_Realization ;
	owl:inverseOf diggr:developedBy ;
	rdfs:comment "A company entity is a developer of a specific edition."@en ;
	rdfs:label "is developer of"@en .

diggr:isPublisherOf a owl:ObjectProperty ;
	rdfs:domain diggr:Company ;
	rdfs:range diggr:LocalRelease ;
	owl:inverseOf diggr:publishedBy ;
	rdfs:comment "A company entity is a publisher of a specific local release."@en ;
	rdfs:label "is publisher of"@en .

diggr:developedBy a owl:ObjectProperty ;
	rdfs:domain diggr:Platform_Realization;
	rdfs:range diggr:Company ;
	owl:inverseOf diggr:isDeveloperOf ;
	rdfs:comment "A platform realization entity is developed by a company entity. (role shortcut)"@en ;
	rdfs:label "developed by"@en .

diggr:portedBy a owl:ObjectProperty ;
	rdfs:domain diggr:Platform_Realization ;
	rdfs:range diggr:Company ;
	rdfs:comment "A platform realization entity is ported by a company entity. (role shortcut)"@en ;
	rdfs:label "ported by"@en .

diggr:publishedBy a owl:ObjectProperty ;
	rdfs:domain diggr:LocalRelease ;
	rdfs:range diggr:Company ;
	owl:inverseOf diggr:isPublisherOf ;
	rdfs:comment "A company entity is a publisher of a specific local release or game. (role shortcut)"@en ;
	rdfs:label "published by"@en .

# distributedBy?

diggr:isInvolvedIn a owl:ObjectProperty ;
	rdfs:domain crm:E39_Actor ;
	rdfs:range diggr:ProductionEvent ;
	rdfs:comment "Persons or companies are involved in the production event of a video game."@en ;
	rdfs:label "is involved in"@en .

diggr:isPortOf a owl:ObjectProperty ;
	rdfs:domain diggr:Platform_Realization ;
	rdfs:range diggr:Platform_Realization ;
	rdfs:comment "A Platform Realization of a game can be a port of a game from another hardware platform."@en ;
	rdfs:label "is port of"@en .

diggr:hasSpecialEdition a owl:ObjectProperty ;
	rdfs:domain diggr:Generic_Edition ;
	rdfs:comment "Another edition of a game can be in some way different from a generic edition of a game, e.g. Gold Edition, Day One Edition, etc."@en ;
	rdfs:label "is special edition of"@en .

diggr:isReleaseOf a owl:ObjectProperty ;
	rdfs:domain diggr:LocalRelease ;
	owl:inverseOf diggr:hasRelease ;
	rdfs:comment "A local release is a specific release of an Edition and a specific Platform Realization."@en ;
	rdfs:label "is release of"@en .

diggr:hasRelease a owl:ObjectProperty ;
	rdfs:range diggr:LocalRelease ;
	owl:inverseOf diggr:isReleaseOf ;
	rdfs:comment "An edition has a specific local release."@en ;
	rdfs:label "has release"@en .

diggr:isEditionOf a owl:ObjectProperty ;
	rdfs:domain diggr:Generic_Edition ;
	owl:inverseOf diggr:hasEdition ;
	rdfs:comment "..."@en ;
	rdfs:label "is edition of"@en .

diggr:hasEdition a owl:ObjectProperty ;
	rdfs:range diggr:Generic_Edition ;
	owl:inverseOf diggr:isEditionOf ;
	rdfs:comment "..."@en ;
	rdfs:label "has edition"@en .

diggr:isPlatformRealizationOf a owl:ObjectProperty ;
	rdfs:domain diggr:Platform_Realization ;
	owl:inverseOf diggr:hasPlatformRealization ;
	rdfs:comment "..."@en ;
	rdfs:label "is platform realization of"@en .

diggr:hasPlatformRealization a owl:ObjectProperty ;
	rdfs:range diggr:Platform_Realization ;
	owl:inverseOf diggr:isPlatformRealizationOf ;
	rdfs:comment "..."@en ;
	rdfs:label "has platform realization"@en .

diggr:releaseCountry a owl:ObjectProperty ;
	rdfs:domain diggr:LocalRelease ;
	rdfs:range gndo:PlaceOrGeographicName ;
	rdfs:comment "The release country or region of a local release."@en ;
	rdfs:label "release country"@en .

diggr:platform a owl:ObjectProperty ;
	rdfs:domain diggr:Platform_Realization ;
	rdfs:range diggr:Platform ;
	rdfs:comment "Relationship to a specific hardware platform."@en ;
	rdfs:label "on/for platform"@en .

## Company Properties

diggr:placeOfBusiness a owl:ObjectProperty ;
    rdfs:domain diggr:Company ;
    rdfs:comment "The place where the headquarter of a company is located." ;
    rdfs:label "place of business"@en .


######################## Datatype Properties #####################################

diggr:hasNote a owl:DatatypeProperty ;
	rdfs:label "has note"@en ;
    rdfs:domain diggr:DiggrEntity .

diggr:releaseDate a owl:DatatypeProperty ;
	rdfs:label "release date"@en ;
	rdfs:comment "The release date of a game entity."@en ;
	rdfs:domain diggr:DiggrEntity .

diggr:variantTitle a owl:DatatypeProperty ;
	rdfs:label "variant title"@en ;
	rdfs:comment "A variant title of something."@en ;
	rdfs:domain diggr:DiggrEntity .
	
diggr:title a owl:DatatypeProperty ;
	rdfs:label "title"@en ;
	rdfs:comment "The title of a game entity."@en ;
	rdfs:domain diggr:DiggrEntity .
	
# genre as a datatype property - maybe later a class with properties: preferredLabel, alternativeLabel,...
diggr:gameGenre a owl:DatatypeProperty ;
	rdfs:label "game genre"@en ;
	rdfs:comment "The categorization of a video game e.g. puzzle video game or dungeon crawl."@en ;
	rdfs:domain diggr:Game .
